dw: test target

dw/DeepWeb/Spec/macros.h
@@ -1,0 +1,7 @@
+#ifndef _Nullable
+#define _Nullable
+#endif
+
+#ifndef _Nonnull
+#define _Nonnull
+#endif
