dw/DeepWeb/Spec/main.c
@@ -1,0 +1,595 @@
+/*
+  This program implements a swap server that accepts connections from multiple
+  clients. On each connection, the server receives bytes from the corresponding
+  client until the buffer is full, at which point the received bytes are deemed
+  a "message". The server replies to this client with the last obtained
+  message, which could have been obtained from another client (on another
+  connection). This last obtained message is initially set to all zeroes.
+
+  All these actions (accepting a new connection, receiving a message, and
+  sending a message) are interleaved.
+ */
+
+#include "macros.h"
+#include <stdlib.h>
+#include <string.h>
+#include <unistd.h>
+#include <netinet/in.h>
+#include <sys/time.h>
+#include <sys/types.h>
+#include <sys/select.h>
+#include <sys/socket.h>
+#include <stdio.h>
+
+#define BUFFER_SIZE 1024
+#define INVALID_SOCKET -1
+
+typedef int socket_fd;
+
+typedef enum state {
+  RECVING,
+  SENDING,
+  DONE,
+  DELETED,
+} state;
+
+typedef struct connection {
+  socket_fd fd;
+  uint32_t request_len;
+  uint8_t request_buffer[BUFFER_SIZE];
+  uint32_t response_len;
+  uint8_t response_buffer[BUFFER_SIZE];
+  uint32_t num_bytes_sent;
+  enum state st;
+  struct connection* next;
+#ifdef DEBUG
+  int connection_id;
+#endif
+} connection;
+
+typedef struct store {
+  uint32_t stored_msg_len;
+  uint8_t stored_msg[BUFFER_SIZE];
+} store;
+
+
+int recv_msg(int fd, uint8_t* buffer_ptr, uint32_t len, int flags) {
+  return recv(fd, buffer_ptr, len, flags);
+}
+
+int send_msg(int fd, uint8_t* buffer_ptr, uint32_t len, int flags) {
+  return send(fd, buffer_ptr, len, flags);
+}
+
+void fd_zero_macro(fd_set* set) {
+  FD_ZERO(set);
+}
+
+int fd_isset_macro(int fd, fd_set* set) {
+  return FD_ISSET(fd, set);
+}
+
+void fd_clr_macro(int fd, fd_set* set) {
+  FD_CLR(fd, set);
+}
+
+void fd_set_macro(int fd, fd_set* set) {
+  FD_SET(fd, set);
+}
+
+static int check_if_complete(uint8_t* buffer_ptr, uint32_t len) {
+  if (BUFFER_SIZE == len) {
+    return 1;
+  }
+
+  return 0;
+}
+
+static connection* new_connection() {
+  connection* result = (connection* )malloc(sizeof(connection));
+  if(result == NULL) {
+    return result;
+  }
+  result->fd = 0;
+  result->request_len = 0;
+  result->response_len = 0;
+  result->num_bytes_sent = 0;
+  result->st = RECVING;
+  result->next = NULL;
+#ifdef DEBUG
+  static int next_cid = 0;
+  result->connection_id = next_cid++;
+#endif
+  return result;
+}
+
+static store* new_store() {
+  store* result = (store* )malloc(sizeof(store));
+  if(result == NULL) {
+    return result;
+  }
+  result->stored_msg_len = 0;
+  uint8_t* buffer = result->stored_msg;
+  memset(buffer, 0, BUFFER_SIZE);
+  return result;
+}
+
+
+/*
+  [populate_response] performs the swap: it populates the response buffer in
+  [conn] with the last stored message, and updates the last stored message
+  to be the message received on this connection (stored in its request buffer).
+ */
+static int
+populate_response(connection* conn, store* last_msg_store) {
+
+  uint8_t* last_msg = last_msg_store->stored_msg;
+  uint32_t last_msg_len = last_msg_store->stored_msg_len;
+
+  // populate response
+  conn->num_bytes_sent = 0;
+  conn->response_len = last_msg_len;
+  uint8_t* response_buffer = conn->response_buffer;
+
+  memcpy(response_buffer, last_msg, last_msg_len);
+
+  // now save the request
+  uint32_t request_len = conn->request_len;
+  last_msg_store->stored_msg_len = request_len;
+
+  uint8_t* request_buffer = conn->request_buffer;
+  memcpy(last_msg, request_buffer, request_len);
+  return 1;
+}
+
+static int
+conn_read(connection* conn, store* last_msg_store) {
+  int r;
+
+  socket_fd conn_fd = conn->fd;
+  uint32_t request_len = conn->request_len;
+  uint8_t* request_buffer = conn->request_buffer;
+
+  uint8_t* ptr = request_buffer + request_len;
+  r = recv_msg(conn_fd, ptr, BUFFER_SIZE - request_len, 0);
+  uint32_t new_len;
+
+  if (r < 0) {
+    return 0;
+  }
+
+  if (r == 0) {
+#ifdef DEBUG
+    printf("conn_read(%d): DELETED\n", conn->connection_id);
+#endif
+
+    conn->st = DELETED; // mark for cleanup later
+    return 0;
+  }
+
+#ifdef DEBUG
+  printf("conn_read(%d): Received %d bytes\n", conn->connection_id, r);
+#endif
+
+  new_len = request_len + r;
+  conn->request_len = new_len;
+
+  int complete = check_if_complete(request_buffer, new_len);
+  if (complete == 0) {
+    return 0;
+  }
+
+  int response_ok = 0;
+  response_ok = populate_response(conn, last_msg_store);
+  if (response_ok == 0) {
+    // fatal error
+    conn->st = DELETED;
+    return 0;
+  }
+
+  // printf("conn_read: Transiting to SENDING\n");
+
+  conn->st = SENDING;
+  return 0;
+}
+
+static void reset_connection(connection* conn, socket_fd fd) {
+
+  uint8_t* request = conn->request_buffer;
+  uint8_t* response = conn->response_buffer;
+
+  conn->fd = fd;
+  conn->st = RECVING;
+  conn->response_len = 0;
+  conn->num_bytes_sent = 0;
+  conn->request_len = 0;
+  memset(request, 0, BUFFER_SIZE);
+  memset(response, 0, BUFFER_SIZE);
+}
+
+static int conn_write(connection* conn) {
+  int r;
+
+  socket_fd conn_fd = conn->fd;
+  uint32_t response_len = conn->response_len;
+  uint32_t num_bytes_sent = conn->num_bytes_sent;
+  uint8_t* response = conn->response_buffer + num_bytes_sent;
+  uint32_t num_bytes_to_send = response_len - num_bytes_sent;
+
+  r = send_msg(conn_fd, response, num_bytes_to_send, 0);
+
+#ifdef DEBUG
+  printf("conn_write(%d): Sent %d bytes\n", conn->connection_id, num_bytes_to_send);
+#endif
+
+  if(r < 0) {
+    conn->st = DELETED; // client possibly disconnected
+    return 0;
+  }
+
+  conn->num_bytes_sent = num_bytes_sent + r;
+
+  if(r < num_bytes_to_send) {
+    return 0;
+  }
+
+  // reset
+  reset_connection(conn, conn_fd);
+
+  return 0;
+}
+
+static int
+process(connection* conn, store* last_msg_store) {
+
+  int r;
+  state conn_st = conn->st;
+  if(conn_st == RECVING) {
+    return conn_read(conn, last_msg_store);
+  }
+  if(conn_st == SENDING) {
+    return conn_write(conn);
+  }
+
+  return 0;
+}
+
+
+/* [accept_connection] accepts a new connection on the socket, creates a
+   connection structure for it, and links it into the head of the linked list.
+ */
+static int accept_connection(socket_fd socket,
+                             connection** head) {
+  socket_fd fd;
+  connection* conn;
+
+  fd = accept(socket, NULL, NULL);
+  if (fd < 0) {
+    return -1;
+  }
+
+  if (fd >= FD_SETSIZE) {
+    shutdown(fd, SHUT_RDWR);
+    close(fd);
+    return -1;
+  }
+
+  conn = new_connection();
+  if (conn == NULL) {
+    shutdown(fd, SHUT_RDWR);
+    close(fd);
+    return -1;
+  }
+
+#ifdef DEBUG
+  printf("accept -> %d\n", conn->connection_id);
+#endif
+
+  reset_connection(conn, fd);
+
+  connection* old_head = *head;
+  conn->next = old_head;
+  *head = conn;
+
+  return 0;
+}
+
+static int add_to_fd_set(socket_fd fd,
+		  fd_set* set,
+		  socket_fd* max_fd) {
+
+  if (set == NULL) {
+    return -1;
+  }
+
+  if (fd >= FD_SETSIZE) {
+    return -1;
+  }
+  if (fd < 0) {
+    return -1;
+  }
+
+  if (max_fd == NULL) {
+    return -1;
+  }
+  if (fd == INVALID_SOCKET) {
+    return -1;
+  }
+
+  fd_set_macro(fd, set);
+
+  int tmp = *max_fd;
+  if(fd > tmp) {
+    *max_fd = fd;
+  }
+
+  return 0;
+}
+
+static void
+monitor_connections(connection* head, fd_set* rs, fd_set* ws,
+		    socket_fd* max_fd) {
+
+  connection* curr = head;
+  state curr_st;
+  socket_fd curr_fd;
+
+  while (curr != NULL) {
+    curr_st = curr->st;
+    curr_fd = curr->fd;
+
+    if (curr_st == RECVING) {
+      add_to_fd_set(curr_fd, rs, max_fd);
+    }
+
+    if (curr_st == SENDING) {
+      add_to_fd_set(curr_fd, ws, max_fd);
+    }
+    curr = curr->next;
+  }
+
+}
+
+static void
+process_connections(connection *head, fd_set* rs, fd_set* ws,
+		    store* last_msg_store) {
+
+  int socket_ready;
+  connection* curr = head;
+  state curr_st;
+  socket_fd curr_fd;
+
+
+  /*
+    This loop iterates over all [connections] in the list pointed to by [head]
+    and does a [process] step.
+
+    EX prefix : list (connection * sockfd * val),
+    EX suffix : list (connection * sockfd * val),
+    EX st : SocketMap,
+    EX last_msg : string,
+    EX curr_ptr : val, such that
+
+    (1) Memory is laid out as:
+    - SOCKAPI st ;
+      FD_SET Tsh read_set read_set_ptr;
+      FD_SET Tsh write_set write_set_ptr;
+
+      TRACE ( (select_loop
+                 server_addr
+                 BUFFER_SIZE
+                 (true, (map proj_conn (prefix ++ suffix), last_msg)))
+                ;; k );
+
+      lseg LS Tsh Tsh (map rep_full_conn prefix) head_ptr curr_ptr;
+      lseg LS Tsh Tsh (map rep_full_conn suffix) curr_ptr nullval;
+      field_at Tsh (Tstruct _store noattr) [] (rep_store last_msg)
+               msg_store_ptr
+
+    (2) The following properties all hold:
+    - consistent_world st
+    - lookup_socket st server_fd = ListeningSocket server_addr
+    - Forall (fun '(conn, fd, ptr) =>
+        consistent_state BUFFER_SIZE st (conn, fd)) prefix;
+    - Forall (fun '(conn, fd, ptr) =>
+        consistent_state BUFFER_SIZE st (conn, fd)) suffix;
+    - exists old_prefix,
+      - connections = old_prefix ++ suffix
+      - map proj_fd old_prefix = map proj_fd prefix, i.e. fds are never changed
+      - map conn_id
+          (map proj_conn old_prefix) = map conn_id (map proj_conn prefix),
+	i.e. ids are never changed
+      - map proj_ptr old_prefix = map proj_ptr prefix, i.e. pointers are never
+        changed.
+    - NoDup
+        (map conn_id
+	  (map proj_conn
+	    (filter
+	      (fun c => (has_conn_state RECVING c
+	        || has_conn_state SENDING c)%bool)
+		(prefix ++ suffix)))), i.e. connection ids among
+      RECVING/SENDING connections are distinct.
+
+   */
+  while (curr != NULL) {
+    curr_fd = curr->fd;
+    int read_socket_ready = fd_isset_macro(curr_fd, rs);
+    int write_socket_ready = fd_isset_macro(curr_fd, ws);
+    socket_ready = 0;
+    if (read_socket_ready) {
+      socket_ready = 1;
+    }
+    else if (write_socket_ready) {
+      socket_ready = 1;
+    }
+
+    if (socket_ready > 0) {
+      process(curr, last_msg_store);
+    }
+    curr = curr->next;
+  }
+
+}
+
+
+int select_loop(socket_fd server_socket, store* last_msg_store) {
+  fd_set rs, ws, es;
+  struct timeval timeout;
+
+  connection *head = NULL;
+  socket_fd maxsock = INVALID_SOCKET;
+
+  timeout.tv_sec = 0;
+  timeout.tv_usec = 0;
+
+  head = NULL;
+
+  /*
+    In this loop, [head] is a pointer to a linked list of connection
+    structures. In each iteration, a new connection is accepted if one is
+    pending on the server socket, and work is performed for each connection
+    in the linked list depending on its state.
+
+    EX connections: list (connection * sockfd * val),
+    EX last_msg : string,
+    EX st : SocketMap,
+    EX read_set : FD_Set,
+    EX write_set : FD_Set,
+    EX exception_set : FD_Set,
+    EX head_ptr : val, such that
+
+    (1) Memory is laid out as:
+    - SOCKAPI st ;
+      FD_SET Tsh read_set v_rs;
+      FD_SET Tsh write_set v_ws;
+      FD_SET Tsh exception_set v_es;
+      ...
+      field_at Tsh (tptr (Tstruct _connection noattr)) [] head_ptr v_head;
+      lseg LS Tsh Tsh
+        (map rep_full_conn connections)
+        head_ptr nullval;
+      ...
+      TRACE (r <- select_loop server_addr BUFFER_SIZE
+                    (true, (map proj_conn connections, last_msg))
+		    ;; k);
+      field_at Tsh (Tstruct _store noattr) [] (rep_store last_msg) msg_store_ptr
+
+    (2) The following properties hold:
+    - consistent_world st, i.e. all connected sockets are associated with
+      distinct connection IDs;
+    - lookup_socket st server_fd = ListeningSocket server_addr
+    - Forall (fun '(conn, fd, ptr) => consistent_state BUFFER_SIZE st (conn, fd))
+        connections, i.e. all connections in the list are "consistent"
+    - NoDup (map descriptor (map proj_fd connections)), i.e. all file
+      descriptors in the list are distinct.
+    - NoDup (map conn_id
+              (map proj_conn
+	        (filter
+		  (fun c => (has_conn_state RECVING c)
+		    || (has_conn_state SENDING c))%bool
+		    connections))),
+      i.e. connection IDs associated with RECVING/SENDING connection structures
+      are distinct.
+   */
+
+  while (1 == 1) {
+    fd_zero_macro(&rs);
+    fd_zero_macro(&ws);
+    fd_zero_macro(&es);
+
+    maxsock = INVALID_SOCKET;
+
+    add_to_fd_set(server_socket, &rs, &maxsock);
+
+    connection* tmp_head = head;
+
+    // loop through all connections in the list to add file descriptors
+    // to the fdsets
+    monitor_connections(tmp_head, &rs, &ws, &maxsock);
+
+    int tmp = maxsock;
+
+    int num_ready = select(tmp + 1, &rs, &ws, &es, &timeout);
+    if (num_ready <= 0) {
+      continue;
+    }
+
+    int socket_ready = fd_isset_macro(server_socket, &rs);
+
+    if (socket_ready) {
+      accept_connection(server_socket, &head);
+      // printf("New connection accepted\n");
+    }
+
+    tmp_head = head;
+
+    // loop through all connections in the list to perform work if needed
+    process_connections(tmp_head, &rs, &ws, last_msg_store);
+
+  }
+
+  return 0;
+}
+
+static void zeroize_addr(struct sockaddr_in* addr) {
+  memset(addr, 0, sizeof(struct sockaddr_in));
+}
+
+static int bind_socket(socket_fd fd, int port) {
+
+  struct sockaddr_in addr;
+  zeroize_addr(&addr);
+
+  int addr_len = sizeof(struct sockaddr_in);
+  addr.sin_family = AF_INET;
+  addr.sin_port = htons(port);
+
+  int r = bind(fd, (struct sockaddr* )&addr, addr_len);
+  if(r < 0) {
+    return -1;
+  }
+
+  return 0;
+}
+
+static void init_store(store* last_msg_store) {
+  last_msg_store->stored_msg_len = BUFFER_SIZE;
+  char* last_msg = (char* )last_msg_store->stored_msg;
+  memset(last_msg, '0', BUFFER_SIZE);
+}
+
+int main(int argc, char** argv) {
+
+  socket_fd fd;
+  int r;
+
+  store* last_msg_store = new_store();
+  if(last_msg_store == NULL) {
+    exit(0);
+  }
+
+  init_store(last_msg_store);
+
+  fd = socket(AF_INET, SOCK_STREAM, 0);
+  if (fd < 0) {
+    exit(0);
+  }
+
+  if (fd >= FD_SETSIZE) {
+    exit(0);
+  }
+
+  int port = 8000;
+  r = bind_socket(fd, port);
+  if (r < 0) {
+    exit(0);
+  }
+
+  r = listen(fd, SOMAXCONN);
+  if (r < 0) {
+    exit(0);
+  }
+
+  // printf("Entering loop...\n");
+  select_loop(fd, last_msg_store);
+}
