dw/DeepWeb/Lib/SimpleSpec.v
@@ -14,14 +14,19 @@ From DeepWeb Require Export
      Lib.SimpleSpec_Descramble
      Lib.SimpleSpec_ServerTrace.
 
+(* SHOW *)
 (* SimpleSpec Interface. *)
 
-(* Module to define servers. *)
+(* Module to define servers. For more details, see
+   [Lib.SimpleSpec_NetworkInterface]. *)
 Module Type NetworkIface.
 
 (* A server is a program with internal nondeterminism and
    external network effects. *)
 Parameter serverE : Type -> Type.
+
+(* Internal nondeterminism is implemented via [nondetE]. *)
+Declare Instance nondet_server : nondetE -< serverE.
 
 (* Accept a new connection. *)
 Parameter accept : M serverE connection_id.
@@ -41,14 +46,19 @@ Parameter recv_full : connection_id -> nat -> M serverE bytes.
 (* Send all bytes in a bytestring. *)
 Parameter send : connection_id -> bytes -> M serverE unit.
 
-(* TODO: null terminated strings? *)
-
 End NetworkIface.
 
-(* Module to define specifications as observers. *)
+(* Module to define specifications as "observers".
+   For more details, see [Lib.SimpleSpec_Observer]. *)
 Module Type ObserverIface.
 
+(* The interface of observer is similar to servers;
+   the difference is that observers only consume bytes,
+   while servers can produce bytes with [send]. *)
 Parameter specE : Type -> Type.
+
+(* Internal nondeterminism is implemented via [nondetE]. *)
+Declare Instance nondet_spec : nondetE -< specE.
 
 (* Observe a new connection. *)
 Parameter obs_connect : M specE connection_id.
@@ -59,6 +69,7 @@ Parameter obs_to_server : connection_id -> M specE byte.
 (* Observe a byte sent from the server. A [None] result is a
    "hypothetical" byte of unknown value (a hole in the observed
    trace). *)
+(* BCP: We'll need some examples showing how the option is handled *)
 Parameter obs_from_server : connection_id -> M specE (option byte).
 
 (* Make an assertion on a value, if it exists. *)
@@ -68,21 +79,84 @@ Parameter assert_on :
 (* Observe a fixed-length message sent to the server. *)
 Parameter obs_msg_to_server : nat -> connection_id -> M specE bytes.
 
-(* Observe a complete message received from the server. *)
+(* Observe a complete message received from the server and match
+   it with an expected value, failing if they are not equal. *)
 Parameter obs_msg_from_server :
   connection_id -> bytes -> M specE unit.
 
 End ObserverIface.
 
-(* Module to connect servers and observers. *)
-Module Type TraceCheck.
+Module Type Traces.
+
+(* An event can be observed to happen on the network,
+   either from the server's or the client's point of view.
+   It is paremeterized by the type to represent the server's
+   output... *)
+Inductive event (byte' : Type) :=
+| NewConnection : connection_id -> event byte'
+| ToServer : connection_id -> byte -> event byte'
+| FromServer : connection_id -> byte' -> event byte'
+.
+
+(* ... In the real world, this output is a concrete byte. *)
+Definition real_event := event byte.
+
+(* ... but it will also be useful for testing to insert hypothetical
+   bytes of unknown values in a trace, representing values that the
+   server may have output but which have not reached the client yet. *)
+Definition hypo_event := event (option byte).
+
+Definition real_trace := list real_event.
+Definition hypo_trace := list hypo_event.
+
+Parameter real_to_hypo : real_trace -> hypo_trace.
+
+Parameter is_server_trace : itree_server -> real_trace -> Prop.
+Parameter is_spec_trace : itree_spec -> hypo_trace -> Prop.
+
+(* Corresponding "server-side" and "client-side" traces. *)
+Parameter network_scrambled : real_trace -> real_trace -> Prop.
+
+(* Property that a real trace [tr] is a scrambled trace of some
+   spec trace. *)
+Definition is_scrambled_trace : itree_spec -> real_trace -> Prop :=
+  fun spec tr =>
+    exists str,
+      network_scrambled str tr /\
+      is_spec_trace spec (real_to_hypo str).
+
+(* Partial test results. *)
+Inductive result' yes no :=
+| Yes (example : yes)
+| No (counterexample : no)
+| Don'tKnow.
+
+Definition result := result' unit unit.
+Definition descrambled_result := result' hypo_trace unit.
+
+(* A test for [is_spec_trace]. *)
+Parameter is_spec_trace_of : nat -> itree_spec -> hypo_trace -> result.
+
+(* A test for [is_scrambled_trace]. Note that the result is
+   a [hypo_trace], and there may be no way to fill the holes
+   to actually satisfy [is_scrambled_trace]. (This test
+   is unsound.) *)
+Parameter is_scrambled_trace_of :
+  nat -> itree_spec -> real_trace -> descrambled_result.
+
+(* Check that every trace of the server can be descrambled into
+   a trace of the spec. *)
 Parameter check_trace_incl_def :
   M specE unit -> M serverE unit -> Checker.
-End TraceCheck.
+
+End Traces.
+(* /SHOW *)
 
 Module Observer : ObserverIface.
 Import Lib.SimpleSpec_Observer.
 Definition specE := specE.
+Instance nondet_spec : nondetE -< specE.
+Proof. typeclasses eauto. Defined.
 Definition obs_connect := @obs_connect specE _.
 Definition obs_to_server := @obs_to_server specE _.
 Definition obs_from_server := @obs_from_server specE _.
