dw/DeepWeb/Test/Client.v
@@ -13,8 +13,9 @@ Parameter file_descr : Type.
 
 Parameter close  : file_descr -> unit.
 Parameter init   : forall {A}, A -> A.
+Parameter log    : string -> unit.
 Parameter recvb  : file_descr -> option byte.
-Parameter sendb  : file_descr -> byte -> unit.
+Parameter sendb  : file_descr -> byte -> nat.
 Parameter socket : unit -> file_descr.
 
 Extract Constant file_descr => "Unix.file_descr".
@@ -25,6 +26,18 @@ Extract Constant init => "fun x ->
   ignore (Unix.system ""make server"");
   Unix.sleep 1;
   x".
+Extract Constant log => "fun cl ->
+  let str =
+    Bytes.to_string (
+      let s = Bytes.create (List.length cl) in
+      let rec copy i = function
+      | [] -> s
+      | c :: l -> Bytes.set s i c; copy (i+1) l
+      in copy 0 cl) in
+  let out = open_out_gen [Open_wronly; Open_append; Open_creat; Open_text]
+                0o666 ""/tmp/client_log"" in
+  output_string out (str ^ ""\n"");
+  close_out out".
 Extract Constant recvb  => "fun sock ->
   let bs = Bytes.create 1 in
   match Unix.recv sock bs 0 1 [] with
@@ -37,7 +50,7 @@ Extract Constant recvb  => "fun sock ->
      else
        None".
 Extract Constant sendb  => "fun sock c ->
-  ignore (Unix.send sock (Bytes.make 1 c) 0 1)".
+  Unix.send sock (Bytes.make 1 c) 0 1 []".
 Extract Constant socket => "fun _ ->
   let open Unix in
   let sock = socket PF_INET SOCK_STREAM 0 in
