dw/DeepWeb/Test/ExternalTest.v
@@ -1,6 +1,6 @@
 Typeclasses eauto := 3.
 
-From Coq Require Import Basics List ZArith.
+From Coq Require Import Basics String List ZArith.
 From ExtLib Require Import Functor OptionMonad StateMonad.
 From QuickChick Require Import QuickChick.
 From DeepWeb Require Import
@@ -25,14 +25,42 @@ Definition recv_external (cid_fd : connection_id * file_descr) : option event :=
 
 Definition Client := state (list (connection_id * file_descr)).
 
+Definition pick_error {A} (l : list A) : option A :=
+  match l with
+  | [] => None
+  | a0::_ => Some (nth (rand (length l)) l a0)
+  end.
+
+Definition pick {A} (l : list A) (a0 : A) : A :=
+  match pick_error l with
+  | None => a0
+  | Some a => a
+  end.
+
+Definition max_connections : nat := 4.
+
 Definition newConnection : Client (connection_id * file_descr) :=
+  ret (log ("new connection"));;
   connections <- get;;
-  let c := (Connection (length connections), socket tt) in
-  put (c :: connections);;
-  ret c.
+  match connections with
+  | [] =>
+    let c := (Connection (length connections), socket tt) in
+    put [c];;
+    ret c
+  | c0::_ =>
+    if length connections <? max_connections
+    then
+      let c := (Connection (length connections), socket tt) in
+      put (c :: connections);;
+      ret (pick connections c)
+    else
+      ret (pick connections c0)
+  end.
 
 Definition sendMessage (b : byte) : Client event :=
+  ret (log ("sending " ++ show b));;
   connections <- get;;
+
   match connections with
   | [] => c <- newConnection;;
          ret (sendb (snd c) b);;
@@ -47,40 +75,49 @@ Definition recvMessage (l : list (connection_id * file_descr)) : trace :=
   filterSome (map recv_external l).
 
 Definition closeAll : Client (list unit) :=
+  ret (log ("closing all connections"));;
   connections <- get;;
   put [];;
   ret (map (close ∘ snd) connections).
 
 Fixpoint execute' (fuel : nat) (msgs : list byte) : Client trace :=
+  ret (log ("execute " ++ show fuel ++ " " ++ show msgs ++ nl));;
   match fuel with
   | 0 => closeAll;;
         ret []
   | S fuel =>
     match msgs with
     | [] =>
+      ret (log ("nothing to send, receiving messages"));;
       tr <- recvMessage <$> get;;
+      ret (log ("received " ++ show tr));;
       closeAll;;
       ret tr
     | msg::msgs' =>
       if flip tt
       then
+        ret (log "flip true, sending messages");;
         ev <- sendMessage msg;;
         evs <- execute' fuel msgs';;
         ret (ev::evs)
       else
         if flip tt
         then
+          ret (log "flip false-true, receiving messages");;
           connections <- get;;
-          evs <- execute' fuel msgs;;
-          ret ((recvMessage connections) ++ evs)
+          tr <- ret (recvMessage connections);;
+          ret (log ("received " ++ show tr));;
+          tr' <- execute' fuel msgs;;
+          ret (app tr tr')
         else
+          ret (log "flip false-false, creating connection");;
           newConnection;;
           execute' fuel msgs
     end
   end.
 
 Definition execute (msgs : list byte) : Client trace :=
-  init <$> execute' (length msgs * 3) msgs.
+  init <$> execute' 1000 msgs.
 
 Instance Checkable_result : Checkable result :=
   {| checker r :=
